

1. Consider Fokker Planck equation  $\frac{\partial}{\partial t} P(x,t) = -\frac{\partial}{\partial x}(f_p) + \frac{1}{2} \frac{\partial^2}{\partial x^2}(g^2 p)$   
 and  $dx_t = v(x_t, t) dt$  satisfy  $\frac{\partial}{\partial t} P(x,t) = -\frac{\partial}{\partial x}(v p)$  ①

②  $t \in \mathbb{D}$

$$\Rightarrow -\frac{\partial}{\partial x}(v p) = -\frac{\partial}{\partial x}(f p) + \frac{1}{2} \frac{\partial^2}{\partial x^2}(g^2 p)$$

$$\Rightarrow \frac{\partial}{\partial x}(v p) = \frac{\partial}{\partial x}\left(f p - \frac{1}{2} \frac{\partial}{\partial x}(g^2 p)\right)$$

$$\Rightarrow v p = f p - \frac{1}{2} \frac{\partial}{\partial x}(g^2 p)$$

$$\Rightarrow v p = f p - \frac{1}{2} \left[ \frac{\partial}{\partial x}(g^2) \cdot p + g^2 \cdot \frac{\partial}{\partial x}(p) \right]$$

$$\Rightarrow v = f - \frac{1}{2} \left[ \frac{\partial}{\partial x}(g^2) + g^2 \cdot \frac{\partial}{\partial x} \ln p \right]$$

$$\Rightarrow v = f - \frac{1}{2} \left[ \frac{\partial}{\partial x}(g^2) + g^2 \cdot \frac{\partial}{\partial x}(\ln p) \right]$$

$$\therefore dx_t = v dt$$

$$= \left[ f - \frac{1}{2} \frac{\partial}{\partial x} g^2 - \frac{g^2}{2} \frac{\partial}{\partial x}(\ln p) \right] dt$$